src/ml/interpreter.ml
@@ -1,0 +1,7 @@
+
+let interpret (prog:Ollvm_ast.toplevel_entity list) =
+  match CFG.coq_TLE_to_cfg prog with
+  | None -> ()
+  | Some cfg -> ()
+  
+  
