src/coq/Effects.v
@@ -51,7 +51,7 @@ Defined.
 (* Domain of semantics *)
 CoInductive D dvalue X :=
 | Ret : X -> D dvalue X
-| Fin : D dvalue X
+| Fin : dvalue -> D dvalue X
 | Err : D dvalue X 
 | Tau : D dvalue X -> D dvalue X
 | Eff : effects dvalue (D dvalue X) -> D dvalue X
@@ -60,7 +60,7 @@ CoInductive D dvalue X :=
 CoFixpoint d_map {A B dvalue} (f:A -> B) (d:D dvalue A) : D dvalue B :=
   match d with
     | Ret a => Ret (f a)
-    | Fin => Fin
+    | Fin d => Fin d
     | Err => Err
     | Tau d' => Tau (d_map f d')
     | Eff m => Eff (effects_map (d_map f) m)
@@ -71,7 +71,7 @@ Section UNFOLDING.
 Definition id_match_d {A dvalue} (d:D dvalue A) : D dvalue A :=
   match d with
     | Ret a => Ret a
-    | Fin => Fin
+    | Fin d => Fin d
     | Err => Err
     | Tau d' => Tau d'
     | Eff m => Eff m
@@ -100,7 +100,7 @@ Definition bind {A B dvalue} (m:D dvalue A) (f:A -> D dvalue B) : D dvalue B :=
   (cofix bindf m:= 
      match m with
        | Ret a => Tau (f a)
-       | Fin => Fin
+       | Fin d => Fin d
        | Err => Err
        | Tau d' => Tau (bindf d')
        | Eff m => Eff (effects_map bindf m)
